---
title: Problem A2 from the 81st Putnam
date: '2022-09-08'
tags: ['Putnam', 'Calculus', 'Math']
draft: false
summary: A solution to a remarkably simple Putnam problem.
---

## Problem

This problem comes from the [81st William Lowell Putnam Mathematical Competition](https://kskedlaya.org/putnam-archive/2020.pdf). 

Let $k$ be a nonnegative integer. Evaluate

$$
\sum_{j=0}^k 2^{k-j} {k+j \choose j}.
$$

## A simplified version

This simplified version was presented as a bonus problem in my multivariable calculus class.

Let 

$$
S_k = \sum_{j=0}^k = 2^{k-j} {k+j \choose j}.
$$

Prove that $S^k = 4^k$ for $k = 0, 1, 2, ...$. 

Hint: 

$$
{k+j \choose j} = \left[ {k+j-1 \choose j} + {k+j-1 \choose j-1} \right]
$$

## Solving the simplified version

The simplified version of this problem can be solved via [proof by induction](https://en.wikipedia.org/wiki/Mathematical_induction). First, we will prove that $S_0 = 4^0$ and then that $S_{k+1} = 4^{k+1}$.

#### $S_0$

$$
S_0 = \sum_{j=0}^0 2^{-j} {j \choose j} = 4^0
$$

#### $S_{k+1}$

$$
S_{k+1} = \sum_{j=0}^{k+1} 2^{k-j+1}{k+j+1 \choose j}
$$

$$
= \sum_{j=0}^{k+1} 2^{k-j+1} \biggl( {k+j \choose j} + {k+j \choose j-1} \biggl)
$$

$$
= \sum_{j=0}^{k+1} 2^{k-j+1} {k+j \choose j} + \sum_{j=0}^{k+1} 2^{k-j+1} {k+j \choose j-1}
$$

$$
= \sum_{j=0}^{k} 2^{k-j+1} + {2k+1 \choose k+1} + \sum_{j=0}^{k} 2^{k-j+1} {k+j \choose j-1} + {2k+1 \choose k}
$$

$$
= 2S_{k} + 2{2k+1 \choose k} + \sum_{j=0}^{k} 2^{k-j+1} {k+j \choose j-1}
$$

$$
= 2S_{k} + 2{2k+1 \choose k} + \sum_{k=0}^{k-1} 2^{k-j} {k+j+1 \choose j}
$$

$$
= 2S_{k} + {2k+1 \choose k} + \sum_{j=0}^{k} 2^{k-j} {k+j+1 \choose k}
$$

$$
=2S_{k} + \frac{1}{2}{2k+1 \choose k+1} + \frac{1}{2}\sum_{j=0}^{k} 2^{k-j+1} {k+j+1 \choose k}
$$

$$
=2S_{k} + \frac{1}{2}\sum_{j=0}^{k+1} 2^{k-j+1} {k+j+1 \choose k}
$$

$$
=2S_{k} + \frac{1}{2}S_{k+1}.
$$

$$
\therefore S_{k+1} = 4S_k = 4^{k+1}
$$
